UniverseAbstractions/Axioms/Universe/StandardEquivalences.lean
@@ -1,0 +1,180 @@
+-- TODO
+#exit
+
+
+
+import UniverseAbstractions.Axioms.Universes
+import UniverseAbstractions.Axioms.Universe.Identity
+import UniverseAbstractions.Axioms.Universe.Functors
+import UniverseAbstractions.Axioms.Universe.Equivalences
+import UniverseAbstractions.Axioms.Universe.Singletons
+import UniverseAbstractions.Axioms.Universe.Products
+import UniverseAbstractions.Lemmas.DerivedFunctors
+import UniverseAbstractions.Lemmas.DerivedSingletonFunctors
+import UniverseAbstractions.Lemmas.DerivedProductFunctors
+
+
+
+--  instance hasLinearCommonEquivalences : HasLinearCommonEquivalences type.{u} :=
+--  { defFunDomainEquiv      := λ e _   => ⟨λ f => funext λ b => congrArg f (e.rightInv b),
+--                                          λ f => funext λ a => congrArg f (e.leftInv  a)⟩,
+--    defFunDomainEquivFun   := λ _ _ _ => HasTrivialFunctoriality.defFun,
+--    defFunCodomainEquiv    := λ e _   => ⟨λ f => funext λ c => e.leftInv  (f c),
+--                                          λ f => funext λ c => e.rightInv (f c)⟩,
+--    defFunCodomainEquivFun := λ _ _ _ => HasTrivialFunctoriality.defFun,
+--    defSwapFunFunEquiv     := λ _ _ _ => ⟨λ _ => funext λ _ => funext λ _ => rfl,
+--                                          λ _ => funext λ _ => funext λ _ => rfl⟩,
+--    defTopElimEquiv        := λ _     => ⟨λ _ => rfl, λ f => funext λ () => rfl⟩,
+--    defProdElimFunEquiv    := λ _ _ _ => ⟨λ _ => funext λ _ => funext λ _ => rfl,
+--                                          λ _ => funext λ (_, _) => rfl⟩,
+--    defProdFstEquiv        := λ e _   => ⟨λ p => prodExt (e.leftInv  p.fst) rfl,
+--                                          λ p => prodExt (e.rightInv p.fst) rfl⟩,
+--    defProdFstEquivFun     := λ _ _ _ => HasTrivialFunctoriality.defFun,
+--    defProdSndEquiv        := λ e _   => ⟨λ p => prodExt rfl (e.leftInv  p.snd),
+--                                          λ p => prodExt rfl (e.rightInv p.snd)⟩,
+--    defProdSndEquivFun     := λ _ _ _ => HasTrivialFunctoriality.defFun,
+--    defProdCommEquiv       := λ _ _   => ⟨λ (_, _) => rfl, λ (_, _) => rfl⟩,
+--    defProdAssocEquiv      := λ _ _ _ => ⟨λ ((_, _), _) => rfl, λ (_, (_, _)) => rfl⟩,
+--    defProdTopEquiv        := λ _     => ⟨λ _ => rfl, λ ((), _) => rfl⟩,
+--    defCompEquivEquiv      := λ e _   => ⟨Equiv.symm_trans_trans e, Equiv.trans_symm_trans e⟩,
+--    defCompEquivEquivFun   := λ _ _ _ => HasTrivialFunctoriality.defFun,
+--    defInvEquivEquiv       := λ _ _   => ⟨Equiv.symm_symm, Equiv.symm_symm⟩ }
+--
+--  instance hasNonLinearCommonEquivalences : HasNonLinearCommonEquivalences type.{u} :=
+--  { defProdDistrEquiv := λ _ _ _ => ⟨λ _ => funext λ _ => prodExt rfl rfl,
+--                                     λ _ => prodExt (funext λ _ => rfl) (funext λ _ => rfl)⟩ }
+--
+--  instance hasBotEquivalences : HasBotEquivalences type.{u} :=
+--  { defBotNotTopEquiv := ⟨λ e => Empty.elim e, λ f => Empty.elim (f ())⟩,
+--    defProdBotEquiv   := λ _ => ⟨λ e => Empty.elim e, λ p => Empty.elim p.fst⟩,
+--    defBotContraEquiv := λ _ => ⟨λ e => Empty.elim e, λ p => Empty.elim (p.snd p.fst)⟩ }
+
+
+
+class HasLinearCommonEquivalences (U : Universe) [HasInternalFunctors U] [HasLinearFunOp U]
+                                  [HasInternalTop U] [HasInternalProducts U] [HasEquivOp U] where
+(defFunDomainEquiv      {A B : U} (E : A ⟷ B) (C : U) :
+   (B ⟶ C) ⟷[HasLinearFunOp.compFunFun (HasEquivalences.toFun  E) C,
+             HasLinearFunOp.compFunFun (HasEquivalences.invFun E) C] (A ⟶ C))
+(defFunDomainEquivFun   (A B C : U)                   :
+   (A ⟷ B) ⟶[λ E => defFunDomainEquiv E C] ((B ⟶ C) ⟷ (A ⟶ C)))
+(defFunCodomainEquiv    {A B : U} (E : A ⟷ B) (C : U) :
+   (C ⟶ A) ⟷[HasLinearFunOp.revCompFunFun C (HasEquivalences.toFun  E),
+             HasLinearFunOp.revCompFunFun C (HasEquivalences.invFun E)] (C ⟶ B))
+(defFunCodomainEquivFun (A B C : U)                   :
+   (A ⟷ B) ⟶[λ E => defFunCodomainEquiv E C] ((C ⟶ A) ⟷ (C ⟶ B)))
+(defSwapFunFunEquiv     (A B C : U)                   :
+   (A ⟶ B ⟶ C) ⟷[HasLinearFunOp.swapFunFunFun A B C, HasLinearFunOp.swapFunFunFun B A C] (B ⟶ A ⟶ C))
+(defTopElimEquiv        (A : U)                       :
+   A ⟷[HasInternalTop.elimFunFun A,
+       HasInternalTop.invElimFun A] (HasTop.Top U ⟶ A))
+(defProdElimFunEquiv    (A B C : U)                   :
+   (A ⟶ B ⟶ C) ⟷[HasInternalProducts.elimFunFun A B C,
+                 HasInternalProducts.invElimFunFunFun A B C] (A ⊓ B ⟶ C))
+(defProdFstEquiv        {A B : U} (E : A ⟷ B) (C : U) :
+   A ⊓ C ⟷[HasInternalProducts.replaceFstFun (HasEquivalences.toFun  E) C,
+           HasInternalProducts.replaceFstFun (HasEquivalences.invFun E) C] B ⊓ C)
+(defProdFstEquivFun     (A B C : U)                   :
+   (A ⟷ B) ⟶[λ E => defProdFstEquiv E C] (A ⊓ C ⟷ B ⊓ C))
+(defProdSndEquiv        {A B : U} (E : A ⟷ B) (C : U) :
+   C ⊓ A ⟷[HasInternalProducts.replaceSndFun (HasEquivalences.toFun  E) C,
+           HasInternalProducts.replaceSndFun (HasEquivalences.invFun E) C] C ⊓ B)
+(defProdSndEquivFun     (A B C : U)                   :
+   (A ⟷ B) ⟶[λ E => defProdSndEquiv E C] (C ⊓ A ⟷ C ⊓ B))
+(defProdCommEquiv       (A B : U)                     :
+   A ⊓ B ⟷[HasInternalProducts.commFun A B, HasInternalProducts.commFun B A] B ⊓ A)
+(defProdAssocEquiv      (A B C : U)                   :
+   (A ⊓ B) ⊓ C ⟷[HasInternalProducts.assocLRFun A B C, HasInternalProducts.assocRLFun A B C] A ⊓ (B ⊓ C))
+(defProdTopEquiv        (A : U)                       :
+   A ⟷[HasInternalProducts.prodTopIntroFun A,
+       HasInternalProducts.prodTopElimFun A] HasTop.Top U ⊓ A)
+(defCompEquivEquiv      {A B : U} (E : A ⟷ B) (C : U) :
+   (B ⟷ C) ⟷[HasEquivOp.compEquivFun E C, HasEquivOp.compEquivFun (HasEquivOp.invEquiv E) C] (A ⟷ C))
+(defCompEquivEquivFun   (A B C : U)                   :
+   (A ⟷ B) ⟶[λ E => defCompEquivEquiv E C] ((B ⟷ C) ⟷ (A ⟷ C)))
+(defInvEquivEquiv       (A B : U)                     :
+   (A ⟷ B) ⟷[HasEquivOp.invEquivFun A B, HasEquivOp.invEquivFun B A] (B ⟷ A))
+
+namespace HasLinearCommonEquivalences
+
+  variable {U : Universe.{u}} [HasInternalFunctors U] [HasLinearFunOp U] [HasInternalTop U]
+           [HasInternalProducts U] [HasEquivOp U] [HasLinearCommonEquivalences U]
+
+  @[reducible] def funDomainEquiv {A B : U} (E : A ⟷ B) (C : U) : (B ⟶ C) ⟷ (A ⟶ C) := defFunDomainEquiv E C
+  @[reducible] def funDomainEquivFun (A B C : U) : (A ⟷ B) ⟶ ((B ⟶ C) ⟷ (A ⟶ C)) := defFunDomainEquivFun A B C
+  @[reducible] def funCodomainEquiv {A B : U} (E : A ⟷ B) (C : U) : (C ⟶ A) ⟷ (C ⟶ B) := defFunCodomainEquiv E C
+  @[reducible] def funCodomainEquivFun (A B C : U) : (A ⟷ B) ⟶ ((C ⟶ A) ⟷ (C ⟶ B)) := defFunCodomainEquivFun A B C
+  @[reducible] def swapFunFunEquiv (A B C : U) : (A ⟶ B ⟶ C) ⟷ (B ⟶ A ⟶ C) := defSwapFunFunEquiv A B C
+
+  @[reducible] def topElimEquiv (A : U) : A ⟷ (HasTop.Top U ⟶ A) := defTopElimEquiv A
+
+  @[reducible] def prodElimFunEquiv (A B C : U) : (A ⟶ B ⟶ C) ⟷ (A ⊓ B ⟶ C) := defProdElimFunEquiv A B C
+  @[reducible] def prodFstEquiv {A B : U} (E : A ⟷ B) (C : U) : A ⊓ C ⟷ B ⊓ C := defProdFstEquiv E C
+  @[reducible] def prodFstEquivFun (A B C : U) : (A ⟷ B) ⟶ (A ⊓ C ⟷ B ⊓ C) := defProdFstEquivFun A B C
+  @[reducible] def prodSndEquiv {A B : U} (E : A ⟷ B) (C : U) : C ⊓ A ⟷ C ⊓ B := defProdSndEquiv E C
+  @[reducible] def prodSndEquivFun (A B C : U) : (A ⟷ B) ⟶ (C ⊓ A ⟷ C ⊓ B) := defProdSndEquivFun A B C
+  @[reducible] def prodCommEquiv (A B : U) : A ⊓ B ⟷ B ⊓ A := defProdCommEquiv A B
+  @[reducible] def prodAssocEquiv (A B C : U) : (A ⊓ B) ⊓ C ⟷ A ⊓ (B ⊓ C) := defProdAssocEquiv A B C
+  @[reducible] def prodTopEquiv (A : U) : A ⟷ HasTop.Top U ⊓ A := defProdTopEquiv A
+
+  @[reducible] def compEquivEquiv {A B : U} (E : A ⟷ B) (C : U) : (B ⟷ C) ⟷ (A ⟷ C) := defCompEquivEquiv E C
+  @[reducible] def compEquivEquivFun (A B C : U) : (A ⟷ B) ⟶ ((B ⟷ C) ⟷ (A ⟷ C)) := defCompEquivEquivFun A B C
+  @[reducible] def invEquivEquiv (A B : U) : (A ⟷ B) ⟷ (B ⟷ A) := defInvEquivEquiv A B
+
+end HasLinearCommonEquivalences
+
+class HasNonLinearCommonEquivalences (U : Universe) [HasFunOp U] [HasInternalTop U]
+                                     [HasInternalProducts U] [HasEquivOp U] where
+(defProdDistrEquiv (A B C : U) :
+   (A ⟶ B ⊓ C) ⟷[HasInternalProducts.distrFun A B C,
+                 HasInternalProducts.invDistrFunFun A B C] (A ⟶ B) ⊓ (A ⟶ C))
+
+namespace HasNonLinearCommonEquivalences
+
+  variable {U : Universe} [HasFunOp U] [HasInternalTop U] [HasInternalProducts U]
+           [HasEquivOp U] [HasNonLinearCommonEquivalences U]
+
+  @[reducible] def prodDistrEquiv (A B C : U) : (A ⟶ B ⊓ C) ⟷ (A ⟶ B) ⊓ (A ⟶ C):= defProdDistrEquiv A B C
+
+end HasNonLinearCommonEquivalences
+
+class HasBotEquivalences (U : Universe) [HasInternalFunctors U] [HasAffineFunOp U]
+                         [HasInternalTop U] [HasInternalBot U] [HasInternalProducts U]
+                         [HasEquivOp U] where
+(defBotNotTopEquiv         :
+   HasBot.Bot U ⟷[HasInternalBot.elimFun (HasInternalBot.Not (HasTop.Top U)),
+                  HasInternalBot.notTopIntroFun] HasInternalBot.Not (HasTop.Top U))
+(defProdBotEquiv   (A : U) :
+   HasBot.Bot U ⟷[HasInternalBot.elimFun (HasBot.Bot U ⊓ A),
+                  HasInternalProducts.fstFun (HasBot.Bot U) A] HasBot.Bot U ⊓ A)
+(defBotContraEquiv (A : U) :
+   HasBot.Bot U ⟷[HasInternalBot.elimFun (A ⊓ HasInternalBot.Not A),
+                  HasInternalProducts.elimFun (HasInternalBot.contraIntroFun A)] A ⊓ HasInternalBot.Not A)
+
+namespace HasBotEquivalences
+
+  variable {U : Universe} [HasInternalFunctors U] [HasAffineFunOp U] [HasInternalTop U]
+           [HasInternalBot U] [HasInternalProducts U] [HasEquivOp U] [HasBotEquivalences U]
+
+  @[reducible] def botNotTopEquiv : HasBot.Bot U ⟷ HasInternalBot.Not (HasTop.Top U) := defBotNotTopEquiv (U := U)
+  @[reducible] def prodBotEquiv (A : U) : HasBot.Bot U ⟷ HasBot.Bot U ⊓ A := defProdBotEquiv A
+  @[reducible] def botContraEquiv (A : U) : HasBot.Bot U ⟷ A ⊓ HasInternalBot.Not A := defBotContraEquiv A
+
+end HasBotEquivalences
+
+class HasClassicalEquivalences (U : Universe) [HasInternalFunctors U] [HasLinearFunOp U]
+                               [HasInternalBot U] [HasClassicalLogic U]
+                               [HasInternalProducts U] [HasEquivOp U] where
+(defByContradictionEquiv (A : U) :
+   A ⟷[HasInternalBot.notNotFun A,
+       HasClassicalLogic.byContradictionFun A] HasInternalBot.Not (HasInternalBot.Not A))
+
+namespace HasClassicalEquivalences
+
+  variable {U : Universe} [HasInternalFunctors U] [HasLinearFunOp U] [HasInternalBot U]
+           [HasClassicalLogic U] [HasInternalProducts U] [HasEquivOp U] [HasClassicalEquivalences U]
+
+  @[reducible] def byContradictionEquiv (A : U) : A ⟷ HasInternalBot.Not (HasInternalBot.Not A) :=
+  defByContradictionEquiv A
+
+end HasClassicalEquivalences
